update soec

proof/spec/Hash.ec
@@ -6,7 +6,7 @@ require import BitEncoding.
 
 from Jasmin require import JModel.
 
-require import Types Params Util.
+require import Types Params Util Utils Address.
 
 import NBytes.
 
@@ -15,9 +15,11 @@ op Hash : W8.t list -> W8.t list.
 op prf_padding_val : W64.t.
 op prf_kg_padding_val : W64.t.
 op F_padding_val : W64.t.
-op padding_len : int.
+op rand_hash_padding : W64.t = W64.one.
 
+op padding_len : int.
 axiom padding_len_ge0 : 0 <= padding_len.
+
 axiom size_hash (x : W8.t list) :  size (Hash x) = n. 
 
 module Hash = {
@@ -62,6 +64,34 @@ module Hash = {
 
     return r;
   }
+
+  proc rand_hash (_left _right : nbytes, _seed : nbytes, address : adrs) : nbytes * adrs = {
+      var padding : W8.t list;
+      var key : W8.t list;
+      var bitmask_0, bitmask_1 : nbytes;
+      var buf, t : W8.t list; 
+      var addr_bytes : W8.t list;
+      var r : W8.t list;
+    
+      padding <@ Util.w64_to_bytes (rand_hash_padding, padding_len);
+
+      address <- set_key_and_mask address 0;
+      addr_bytes <- addr_to_bytes address;
+      key <@ prf (addr_bytes, _seed);
+
+      address <- set_key_and_mask address 1;
+      addr_bytes <- addr_to_bytes address;
+      bitmask_0 <@ prf (addr_bytes,  _seed);
+
+      address <- set_key_and_mask address 2;
+      addr_bytes <- addr_to_bytes address;
+      bitmask_1 <@ prf (addr_bytes,  _seed);
+    
+      t <- (nbytexor _left bitmask_0) ++ (nbytexor _right bitmask_1);
+      buf <- padding ++ key ++ t;
+  
+      return (Hash buf, address);
+  }
 }.
 
 
@@ -75,3 +105,40 @@ lemma prf_kg_ll : islossless Hash.prf_keygen
 
 lemma f_ll : islossless Hash._F 
     by proc; wp; call w64_to_bytes_ll; skip; smt(padding_len_ge0).
+
+lemma rand_hash_ll : islossless Hash.rand_hash
+    by proc; call f_ll; wp; do ! (call prf_ll; wp); call w64_to_bytes_ll; skip; smt(padding_len_ge0).
+
+(*---------------------------------------------------------------------------------------------------------*)
+
+lemma _prf_size : hoare [Hash.prf : true ==> size res = n].
+proof.
+proc; seq 2 : (true); auto => />; smt(size_hash).
+qed.
+
+lemma prf_size : phoare [Hash.prf : true ==> size res = n] = 1%r 
+    by conseq prf_ll _prf_size => /#.
+
+lemma _prf_keygen_size : hoare [Hash.prf_keygen : true ==> size res = n].
+proof.
+proc; seq 2 : (true); auto => />; smt(size_hash).
+qed.
+
+lemma prf_keygen_size : phoare [Hash.prf_keygen : true ==> size res = n] = 1%r 
+    by conseq prf_kg_ll _prf_keygen_size => /#.
+
+lemma _f_size : hoare [Hash._F : true ==> size res = n].
+proof.
+proc; seq 2 : (true); auto => />; smt(size_hash).
+qed.
+
+lemma f_size : phoare [Hash._F : true ==> size res = n] = 1%r
+    by conseq f_ll _f_size => /#.
+
+lemma _randhash_size : hoare [Hash.rand_hash : true ==> size res.`1 = n]
+    by proc; seq 11 : (true); auto => />; call _f_size; skip => />.
+
+lemma randhash_size : phoare [Hash.rand_hash : true ==> size res.`1 = n] = 1%r
+    by conseq rand_hash_ll _randhash_size => /#.
+
+(*---------------------------------------------------------------------------------------------------------*)
