proof/spec/XMSS_MT_PRF.ec
@@ -4,105 +4,24 @@ require import AllCore List RealExp IntDiv.
 require (*--*) Subtype. 
 
 from Jasmin require import JModel.
-
-require import Params Notation Parameters Address Primitives Wots.
-
-import NBytes.
+ 
+require import Types Params Notation Parameters Address Hash Primitives Wots Util.
+ 
+import NBytes OTSKeys Three_NBytes AuthPath.
 import Array8.
 
-clone import Subtype as Three_NBytes with 
-   type T = W8.t list,
-   op P = fun l => size l = 3 * n
-   rename "T" as "three_n_bytes"
-   proof inhabited by (exists (nseq (3*n) W8.zero);smt(size_nseq ge0_n))
-   proof *.
-
-clone import Subtype as OTSKeys with 
-   type T = wots_sk list,
-   op P = fun l => size l = 2^h
-   rename "T" as "wots_ots_keys".
-
-clone import Subtype as AuthPath with
-  type T = nbytes list,
-  op P = fun l => size l = len
-  rename "T" as "auth_path"
-  proof inhabited by (exists (nseq len (nseq n W8.zero));smt(size_nseq ge0_len))
-  proof *.
-
-op d : { int | 1 <= d } as ge1_d. (* d layers of trees, each having height h/d  *)
-op h : { int | 0 <= h /\ h %% d = 0} as h_vals. (* hyper-tree of total height h, where h is a multiple of d *)
-
 (**********************************************************************************************)
 
-(* gets the n most significant bits *)
-op msb (x : W8.t list) (n : int) : W8.t list = take n x. 
-
-(* gets the n most significant bits of x *)
-(* n is at most 32 *)
-op msb_w32 (x : W32.t) (n : int) : bool list = take n (w2bits x).
-
-(* Returns the n most significant bits of x as a W32.t *)
-op msb_w32_int (x : W32.t) (n : int) : W32.t = 
-  let bits : bool list = take n (w2bits x) in
-  (W32.bits2w bits).
-
-op lsb_w32_int (x : W32.t) (n : int) : W32.t =
-   let bits : bool list =  w2bits x in
-   let lsbits : bool list =  drop ((size bits) - n) bits in
-   W32.bits2w lsbits.
-
-(**********************************************************************************************)
-
-op H : nbytes -> bitmask -> nbytes.
+op H : nbytes -> nbytes -> nbytes.
 op H_msg : three_n_bytes -> W8.t list -> nbytes.
-op _prf_ : nbytes -> W8.t list -> nbytes.
 op impl_oid : W32.t.
 
 (**********************************************************************************************)
 
-type xmss_mt_sk = { idx : W32.t ;
-                    sk_seed : nbytes ; (* secret *)
-                    sk_prf : nbytes ;
-                    pub_seed_sk : nbytes ; (* public *)
-                    sk_root : nbytes }.
-
-type xmss_mt_pk = { pk_oid : W32.t ;
-                    pk_root : nbytes ;
-                    pk_pub_seed : nbytes }.
-
-type msg_t = W8.t list.
-
-type sig_t = { sig_idx : W32.t;
-               r : nbytes;
-               wots_sig : wots_signature;
-               authentication_path : auth_path }.
-
-type xmss_mt_keypair = xmss_mt_sk * xmss_mt_pk.
-
-(**********************************************************************************************)
-
-(* 4.1.4 Randomized tree hashing *)
-module RandHash = {
-proc rand_hash (_left _right : nbytes, _seed : seed, address : adrs) : nbytes * adrs = { 
-  var key : nbytes;
-  var bitmask_0 : nbytes;
-  var bitmask_1 : nbytes;
-  var hash_in : nbytes;
-
-  address <- set_key_and_mask address 0;
-  key <- PRF _seed address;
-  address <- set_key_and_mask address 1;
-  bitmask_0 <- PRF _seed address;
-  address <- set_key_and_mask address 2;
-  bitmask_1 <- PRF _seed address;
-  hash_in <- (nbytexor _left bitmask_0) ++ (nbytexor _right bitmask_1);
-  
-  return (H key hash_in, address);
-  }
-}.
-(**********************************************************************************************)
-
 (* 4.1.5 L-Trees *)
+(* takes as input a WOTS+ public key pk and compresses it to a single 
+   n-byte value pk[0].
+*)
 module LTree = {
   proc ltree (pk : wots_pk, address : adrs, _seed : seed) : nbytes * adrs = {
     var pk_i : nbytes;
@@ -118,7 +37,7 @@ module LTree = {
         address <- set_tree_index address i;
         pk_i <- nth witness pk (2*i);
         tmp <- nth witness pk (2*i + 1);
-        (pk_i, address) <@ RandHash.rand_hash (pk_i, tmp, _seed, address);
+        (pk_i, address) <@ Hash.rand_hash (pk_i, tmp, _seed, address);
         pk <- put pk i pk_i;
       }
 
@@ -138,42 +57,50 @@ module LTree = {
 }. 
 
 
-lemma neg_lt (x y : int) : ! (x < y) <=> y <= x by smt().
-
-
 lemma ltree_ll : islossless LTree.ltree.
 proof.
 proc.
-sp ; wp.
-while (1 <= _len <= len) (_len - 1) ; auto => />.
-- while (0 <= i <= floor (len%r / 2%r)) (floor (len%r / 2%r) - i) ; auto => />.
-  + progress.  admit.
-  + progress; 1,2,3,4,5: by admit.
-- admit. (* split ;  [ smt(ge0_len) | move => * ; rewrite neg_lt /# ]. *)
+islossless.
+while (true) (_len - 1); last by skip => /> /#.
+auto => />.
+while (0 <= _len <= len) (floor (len%r / 2%r) - i).
+auto => />; call rand_hash_ll. wp. skip => /> *. 
+rewrite !negb_and.
+left; left. 
+admit.
+
+auto => /> *. do split. 
+smt(). 
+admit.
+smt().
+move => *. admit.
 qed.
 
+lemma ltree_size : hoare [LTree.ltree : true ==> size res.`1 = n].
+proof.
+proc.
+seq 3 : (true); first by auto.
+seq 1 : (forall (x : W8.t list), x \in pk => size pk = n); last first.
+  + auto => /> &hr *. admit.
+admit.
+qed.
+
+
 (**********************************************************************************************)
-
-(* Stack operations *)
-abbrev push (x : 'a list) (a : 'a) : 'a list = rcons x a. 
-
-op remove_last (x : 'a list) : 'a list = 
-with x = [] => []
-with x = h::t => if t = [] then [] else remove_last t.
-
-abbrev pop (x : 'a list) : 'a list * 'a = 
-    let last_elem : 'a = last witness x in
-    let new_list = remove_last x in
-    (new_list, last_elem).
 
 (* It is REQUIRED that s % 2^t = 0, i.e., that the leaf at index s is a leftmost leaf of a sub-tree of height t. *)
 pred leftmost_leaf (s t : int)  = s %% 2^t = 0.
 
+(* Precondition *)
 pred treehash_p (s t : int) = s %% (1 `<<` t) <> 0.
 
 
-(* NOTE: In the implementation, treehash (in xmss_core.c) computes both the authentication 
+(* NOTE: In the Jasmin implementation, treehash (in xmss_core.c) computes both the authentication 
          path and the resulting root node *)
+(* computation of the internal n-byte nodes of a Merkle tree *)
+(* The treeHash algorithm returns the root node of a tree of height t with the leftmost 
+   leaf being the hash of the WOTS+ pk with index s.  
+*)
 module TreeHash = {
   (* Computes the root *)
   proc treehash(sk : xmss_mt_sk, s t : int, address : adrs) : nbytes * adrs = {
@@ -185,7 +112,7 @@ module TreeHash = {
   var pk : wots_pk;
   var i : int <- 0;
   var tree_index, tree_height: int;
-  var heights : int list;
+  var heights : int list <- nseq (h + 1) 0; (* TODO: Check if this is the correct size *)
   var tmp : int;
   var offset : int <- 0;
     
@@ -220,7 +147,7 @@ module TreeHash = {
         address <- set_tree_index address (ceil((tree_index - 1)%r / 2%r));
         (stack, top_node) <- pop stack;
 
-        (node, address) <@ RandHash.rand_hash (top_node, node, pub_seed, address);
+        (node, address) <@ Hash.rand_hash (top_node, node, pub_seed, address);
         
         (* ----------- not in the RFC ----------- *)
         offset <- offset - 1;
@@ -244,15 +171,18 @@ lemma treehash_ll : islossless TreeHash.treehash.
 proof.
 proc.
 sp ; wp.
-while (true) (2^t - i) ; auto => /> ; last by progress ; rewrite neg_lt /#.
-sp ; wp. 
-admit.
+while (true) (2^t - i); last by skip => /> /#.
+auto => />. sp.
+while (true) (offset - 1).
+  + auto => />; call rand_hash_ll; wp; skip => /> /#.
+  + wp; call ltree_ll; wp; call wots_pkGen_ll; wp. skip => /> *.
+    split; [ move => *; rewrite negb_and; left |]; smt().
 qed.
 
 module TreeSig = {
+  (* Compute the authentication path for the i-th WOTS+ key pair *)
   proc buildAuthPath(sk : xmss_mt_sk, idx : W32.t, address : adrs) : auth_path * adrs = {
-    var authentication_path : auth_path;
-    
+    var authentication_path : auth_path <- nseq len (nseq n W8.zero);
     var j : int <- 0;
     var k : int;
     var t : nbytes <- witness;
@@ -261,14 +191,15 @@ module TreeSig = {
       k <- floor((W32.to_uint idx)%r / (2^j)%r);
       (t, address) <@ TreeHash.treehash(sk, k * (2^j), j, address);
       authentication_path <- put authentication_path j t;
-      j <- j+1;
+      j <- j + 1;
     }
 
     return (authentication_path, address);
   }
 
+  (* Generate a WOTS+ signature on a message with corresponding authentication path *)
   proc treesig(M : nbytes, sk : xmss_mt_sk, idx : W32.t, address : adrs) : wots_signature * auth_path * adrs  = {
-    var auth : auth_path;
+    var auth : auth_path <- nseq len (nseq n W8.zero);
     var sig_ots : wots_signature;
     var ots_sk : wots_sk;
     var seed : nbytes;
@@ -286,48 +217,19 @@ module TreeSig = {
 lemma buildAuthPath_ll : islossless TreeSig.buildAuthPath.
 proof.
 proc.
-while (0 <= j <= h) (h - j) ; auto => />.
-  - call treehash_ll ; auto => /> /#. 
-  - split ; smt(h_vals). 
+while (0 <= j <= h) (h - j) ; auto => />; [call treehash_ll ; auto => /> /# | smt(h_g0) ]. 
 qed.
 
-lemma treesig_ll : islossless TreeSig.treesig.
-proof.
-proc.
-call wots_sign_seed_ll.
-auto => /> ; call buildAuthPath_ll.
-by skip.
-qed.
+lemma treesig_ll : islossless TreeSig.treesig
+    by proc; call wots_sign_seed_ll; auto => /> ; call buildAuthPath_ll; auto.
 
-module XMSS_MT_PRF = {
-   proc kg() : xmss_mt_keypair = {
-      var pk : xmss_mt_pk <- witness;
-      var sk : xmss_mt_sk <- witness;
 
-      var idx_MT : W32.t <- W32.zero;
-      var sk_seed, sk_prf, pub_seed, root : nbytes;
+op append_sig (sig : sig_t) (r_sig : reduced_signature) : sig_t =    
+    let new_sigs: reduced_signature list = sig.`r_sigs ++ [r_sig] in
+    {| sig with  r_sigs=new_sigs|}.
 
-      var address : adrs <- zero_address;
-      
-      sk_seed <$ DList.dlist W8.dword n;
-      sk_prf <$ DList.dlist W8.dword n;
-      pub_seed <$ DList.dlist W8.dword n;
-
-      (root, address) <@ TreeHash.treehash(sk, 0, h, address);
-
-      sk <- {| idx=idx_MT;
-               sk_seed=sk_seed;
-               sk_prf=sk_prf;
-               pub_seed_sk=pub_seed;
-               sk_root=root;
-             |};
-
-      pk <- {| pk_oid=impl_oid; pk_root=root; pk_pub_seed=pub_seed |};
-
-      return (sk, pk);
-   }
-
-   proc rootFromSig(idx_sig : W32.t, sig_ots : wots_signature, auth : auth_path, M : nbytes, 
+module XMSS = {
+  proc rootFromSig(idx_sig : W32.t, sig_ots : wots_signature, auth : auth_path, M : nbytes, 
                    _seed : seed, address : adrs) : nbytes = {
     var pk_ots : wots_pk;
     var k : int <- 0;
@@ -356,13 +258,13 @@ module XMSS_MT_PRF = {
         address <- set_tree_index address (index %/ 2);
 
         auth_k <- nth witness auth k;
-        (nodes1, address) <@ RandHash.rand_hash(nodes0, auth_k, _seed, address);
+        (nodes1, address) <@ Hash.rand_hash (nodes0, auth_k, _seed, address);
       } else {
         index <- get_tree_index address;
         address <- set_tree_index address ((index - 1) %/ 2);
 
         auth_k <- nth witness auth k;
-        (nodes1, address) <@ RandHash.rand_hash(auth_k, nodes0, _seed, address);
+        (nodes1, address) <@ Hash.rand_hash (auth_k, nodes0, _seed, address);
       }
 
       nodes0 <- nodes1;
@@ -372,21 +274,144 @@ module XMSS_MT_PRF = {
     return nodes0;
   }
 
+}.
 
+module XMSS_MT_PRF = {
+   (* Different from the spec because we use a secret seed instead of the full wots keys *)
+   (* Algorithm 10 instead of 15 *)
+   (*
+            +---------------------------------+
+            |          algorithm OID          |     W32 (4 bytes)
+            +---------------------------------+
+            |                                 |
+            |            root node            |     n bytes
+            |                                 |
+            +---------------------------------+
+            |                                 |
+            |              SEED               |     n bytes
+            |                                 |
+            +---------------------------------+
 
+                            XMSS^MT Public Key
+   *)
+   proc kg() : xmss_mt_keypair = {
+      var pk : xmss_mt_pk <- witness;
+      var sk : xmss_mt_sk <- witness;
+
+      var sk_seed, sk_prf, pub_seed, root : nbytes;
+
+      var address : adrs <- zero_address;
+      
+      sk_seed <$ DList.dlist W8.dword n;
+      sk_prf <$ DList.dlist W8.dword n;
+      pub_seed <$ DList.dlist W8.dword n;
+
+      (root, address) <@ TreeHash.treehash(sk, 0, h, address);
+
+      sk <- {| idx=W32.zero;
+               sk_seed=sk_seed;
+               sk_prf=sk_prf;
+               pub_seed_sk=pub_seed;
+               sk_root=root;
+             |};
+
+      pk <- {| pk_oid=impl_oid; pk_root=root; pk_pub_seed=pub_seed |};
+
+      return (sk, pk);
+   }
+
+  
+   (* Algorithm 13 *)
+   proc rootFromSig(idx_sig : W32.t, sig_ots : wots_signature, auth : auth_path, M : nbytes, 
+                   _seed : seed, address : adrs) : nbytes = {
+    var pk_ots : wots_pk;
+    var k : int <- 0;
+    var nodes0, nodes1 : nbytes <- nseq n W8.zero;
+    var index : int;
+    var auth_k : nbytes;
+    
+    address <- set_type address 0;
+    address <- set_ots_addr address (W32.to_uint idx_sig);
+
+    (pk_ots, address) <@ WOTS.pkFromSig(M, sig_ots, _seed, address);
+
+    address <- set_type address 1;
+    address <- set_ltree_addr address (W32.to_uint idx_sig);
+
+    (nodes0, address) <@ LTree.ltree(pk_ots, address, _seed);
+
+    address <- set_type address 2;
+    address <- set_tree_index address (W32.to_uint idx_sig);
+ 
+    while (k < h) {
+      address <- set_tree_height address k;
+
+      if (floor ((W32.to_uint idx_sig)%r / (2^k)%r) %% 2 = 0) {
+        index <- get_tree_index address;
+        address <- set_tree_index address (index %/ 2);
+
+        auth_k <- nth witness auth k;
+        (nodes1, address) <@ Hash.rand_hash(nodes0, auth_k, _seed, address);
+      } else {
+        index <- get_tree_index address;
+        address <- set_tree_index address ((index - 1) %/ 2);
+
+        auth_k <- nth witness auth k;
+        (nodes1, address) <@ Hash.rand_hash(auth_k, nodes0, _seed, address);
+      }
+
+      nodes0 <- nodes1;
+      k <- k+1;
+    }
+
+    return nodes0;
+  }
+
+   (*
+           +---------------------------------+
+           |                                 |
+           |          index idx_sig          |   ceil(h / 8) bytes
+           |                                 |
+           +---------------------------------+
+           |                                 |
+           |          randomness r           |   n bytes
+           |                                 |
+           +---------------------------------+
+           |                                 |
+           |  (reduced) XMSS signature Sig   |   (h / d + len) * n bytes
+           |        (bottom layer 0)         |
+           |                                 |
+           +---------------------------------+
+           |                                 |
+           |  (reduced) XMSS signature Sig   |   (h / d + len) * n bytes
+           |            (layer 1)            |
+           |                                 |
+           +---------------------------------+
+           |                                 |
+           ~              ....               ~
+           |                                 |
+           +---------------------------------+
+           |                                 |
+           |  (reduced) XMSS signature Sig   |   (h / d + len) * n bytes
+           |          (layer d - 1)          |
+           |                                 |
+           +---------------------------------+
+
+                             XMSS^MT Signature
+   *)
    proc sign(sk : xmss_mt_sk, m : msg_t) : sig_t * xmss_mt_sk = {
       var sig : sig_t;
       var idx : W32.t <-sk.`idx;
       var idx_new : W32.t;
       var idx_bytes : W8.t list;
-      var idx_nbytes : nbytes;
+      var idx_nbytes : nbytes <- nseq n W8.zero;
       var idx_tree : W32.t;
       var idx_leaf : W32.t;
-      var _R : nbytes;
-      var _M' : nbytes;
+      var _R : nbytes <- nseq n W8.zero;
+      var _M' : nbytes <- nseq n W8.zero;
       var address : adrs <- zero_address;
       var root : nbytes <- sk.`sk_root;
-      var t : three_n_bytes;
+      var t : three_n_bytes <- nseq (3*n) W8.zero;
       var sk_prf : nbytes <- sk.`sk_prf;
       var j : int;
       var pub_seed : nbytes <- sk.`pub_seed_sk;
@@ -399,10 +424,10 @@ module XMSS_MT_PRF = {
       sk <- {| sk with idx=idx_new |};
 
       idx_bytes <- toByte idx 32;
-      _R <- _prf_ sk_prf idx_bytes;
+      _R <@ Hash.prf(sk_prf, idx_bytes);
 
       idx_nbytes <- toByte idx n;
-      t <- _R ++ root ++ idx_nbytes;
+      t <- _R ++ root ++ idx_nbytes; (* t = r || getRoot(SK_MT) || (toByte(idx_sig, n)) *)
       _M' <- H_msg t m;
 
       idx_tree <- msb_w32_int idx (h - (h %/ d));
@@ -413,7 +438,7 @@ module XMSS_MT_PRF = {
 
       (sig_tmp, auth, address) <@ TreeSig.treesig(_M', sk, idx_leaf, address);
      
-      (* sig <- {| sig with reduced_sig_mt=[(sig_tmp, auth)] |}; *)
+      sig <- {| sig with r_sigs = [(sig_tmp, auth)] |}; (* Sig_MT = Sig_MT || r || Sig_tmp; *)
 
       j <- 1;
       while (j < d) {
@@ -426,9 +451,9 @@ module XMSS_MT_PRF = {
 
       (sig_tmp, auth, address) <@ TreeSig.treesig(root, sk, idx_leaf, address);
       
-      (* sig <- append_sig sig (sig_tmp, auth); *)
+      sig <- append_sig sig (sig_tmp, auth);
       
-      
+       
       j <- j+1;
     }
       
@@ -436,58 +461,58 @@ module XMSS_MT_PRF = {
       return (sig, sk);
    }
 
-  (*
+  (* Algorithm 14 *)
    proc verify(pk : xmss_mt_pk, m : msg_t, s : sig_t) : bool = {
-     var is_valid : bool;
-     (* var idx : W32.t <- s.`sig_idx_mt; *)
-     (* var idx_bytes : nbytes <- toByte idx n; *)
-     var seed : nbytes <- pk.`pk_pub_seed;
-     var address : adrs <- zero_address;
-     (* var idx_leaf : W32.t <- lsb_w32_int idx (h %/ d); *)
-     (* var idx_tree : W32.t <- msb_w32_int idx (h - (h %/ d)); *)
-     (* var _sig : reduced_sig; *)
-     var node, root, _R, _M': nbytes;
-     var t : three_n_bytes;
-     var j : int;
-
-      (* _sig <- nth witness s.`reduced_sig_mt 0; *)
-
-      (* _R <- s.`r_mt; *)
-     root <- pk.`pk_root;
-     t <- _R ++ root ++ idx_bytes;
-      _M' <- H_msg t m; 
+       var is_valid : bool;
+       var idx_sig : W32.t <- s.`sig_idx;
+       var seed : nbytes <- pk.`pk_pub_seed;
+       var idx_bytes : nbytes <- toByte idx_sig n;
+       var node, root, _R, _M': nbytes;
+       var t : three_n_bytes;
+       var address : adrs <- zero_address;
+       var j : int;
      
-     node <@ XMSS.rootFromSig(idx_leaf, _sig.`1, _sig.`2, _M', seed, address);
+       var idx_leaf : W32.t <- lsb_w32_int idx_sig (h %/ d);
+       var idx_tree : W32.t <- msb_w32_int idx_sig (h - (h %/ d));
+     
+       var _sig : reduced_signature <- nth witness s.`r_sigs 0;
+     
+       (* M' = H_msg(getR(Sig_MT) || getRoot(PK_MT) || (toByte(idx_sig, n)), M); *)
+       root <- pk.`pk_root;
+       t <- _R ++ root ++ idx_bytes;
+       _M' <- H_msg t m; 
 
-     j <- 1;
-     while (j < d) {
-       (* idx_leaf <- lsb_w32_int idx_tree (h %/ d); *)
-       (* idx_tree <- msb_w32_int idx_tree (h - (h %/ d)); *)
-
-       (* _sig <- nth witness s.`reduced_sig_mt j; *)
-      
-       address <- set_layer_addr address j;
+       address <- set_layer_addr address 0;
        address <- set_tree_addr address (W32.to_uint idx_tree);
 
        node <@ XMSS.rootFromSig(idx_leaf, _sig.`1, _sig.`2, _M', seed, address);
+     
+       j <- 1;
+       while (j < d) {
+         idx_leaf <- lsb_w32_int idx_tree (h %/ d);
+         idx_tree <- msb_w32_int idx_tree (h - (h %/ d));
 
-       j <- j + 1;
-     }
+         _sig <- nth witness s.`r_sigs j;
 
-    is_valid <- (node = root);
+         address <- set_layer_addr address j;
+         address <- set_tree_addr address (W32.to_uint idx_tree);
+       
+         node <@ XMSS.rootFromSig(idx_leaf, _sig.`1, _sig.`2, _M', node, address);
 
+         j <- j + 1;
+       }
 
-
-     return is_valid;
+       
+           is_valid <- (node = root);
+           return is_valid;
    }
-   *)
 }.
 
 lemma xmss_mt_kg_ll : islossless XMSS_MT_PRF.kg.
 proof.
 proc.
 auto => /> ; call treehash_ll.
-auto => /> *. smt(@Distr @DList @W8).
+auto => /> *; smt(@Distr @DList @W8).
 qed.
 
 lemma root_from_sig_ll : islossless XMSS_MT_PRF.rootFromSig.
@@ -496,7 +521,7 @@ proc.
 while (0 <= k <= h) (h - k) ; auto => />; 1,2:admit. (* by progress ; smt(). *)
 call ltree_ll ; auto => />. 
 call wots_pkFromSig_ll ; auto => />.
-smt(h_vals).
+smt(h_g0).
 qed.
 
 lemma xmss_mt_sign_ll : islossless XMSS_MT_PRF.sign.
@@ -505,7 +530,6 @@ proc.
 while (0 <= j <= d) (d - j) ; auto => />.
   - call treesig_ll ; auto => />. call treehash_ll. skip => /> /#.
   - progress ; smt().
-  - call treesig_ll ; auto => /> ; smt(ge1_d).
-qed.
-
+  - call treesig_ll; wp.  call prf_ll; wp.  skip => />; smt(ge0_d). 
+qed. 
 
