proof/spec/Util.ec
@@ -6,6 +6,47 @@ require import BitEncoding.
 
 from Jasmin require import JModel.
 
+require import Types.
+(*---*) import NBytes.
+
+op nbytexor(a b : nbytes) : nbytes = 
+    map (fun (ab : W8.t * W8.t) => ab.`1 `^` ab.`2) (zip a b).
+
+(******************************************************************************)
+
+(* gets the n most significant bits *)
+op msb (x : W8.t list) (n : int) : W8.t list = take n x. 
+
+(* gets the n most significant bits of x *)
+(* n is at most 32 *)
+op msb_w32 (x : W32.t) (n : int) : bool list = take n (w2bits x).
+
+(* Returns the n most significant bits of x as a W32.t *)
+op msb_w32_int (x : W32.t) (n : int) : W32.t = 
+  let bits : bool list = take n (w2bits x) in
+  (W32.bits2w bits).
+
+op lsb_w32_int (x : W32.t) (n : int) : W32.t =
+   let bits : bool list =  w2bits x in
+   let lsbits : bool list =  drop ((size bits) - n) bits in
+   W32.bits2w lsbits.
+
+(******************************************************************************)
+
+(* Stack operations *)
+op push (x : 'a list) (a : 'a) : 'a list = rcons x a. 
+
+op remove_last (x : 'a list) : 'a list = 
+with x = [] => []
+with x = h::t => if t = [] then [] else remove_last t.
+
+op pop (x : 'a list) : 'a list * 'a = 
+    let last_elem = last witness x in
+    let new_list = remove_last x in
+    (new_list, last_elem).
+
+(******************************************************************************)
+
 module Util = {
   proc w64_to_bytes (in_0 : W64.t, outlen : int) = {
     var r : W8.t list <- nseq outlen W8.zero;
